restructure sha2-vec

code/sha2-vec/Hacl.Impl.SHA2.Core.fst
@@ -9,16 +9,14 @@ open Lib.NTuple
 open Lib.Buffer
 open Lib.IntVector
 open Lib.MultiBuffer
+open Lib.CreateN
 
 open Spec.Hash.Definitions
 open Hacl.Hash.Definitions
 open Hacl.Spec.SHA2.Vec
 
-
 module ST = FStar.HyperStack.ST
 module NTup = Lib.NTuple
-module Constants = Spec.SHA2.Constants
-module Spec = Hacl.Spec.SHA2
 module SpecVec = Hacl.Spec.SHA2.Vec
 module VecTranspose = Lib.IntVector.Transpose
 module LSeq = Lib.Sequence
@@ -26,120 +24,35 @@ module LSeq = Lib.Sequence
 
 #set-options "--max_fuel 0 --max_ifuel 0 --z3rlimit 50"
 
-(** Top-level constant arrays for the SHA2 algorithms. *)
+unfold
+let state_t (a:sha2_alg) (m:m_spec) =
+  lbuffer (element_t a m) 8ul
 
-let h224 : x:glbuffer uint32 8ul{witnessed x Constants.h224 /\ recallable x} =
-  createL_global Constants.h224_l
-let h256 : x:glbuffer uint32 8ul{witnessed x Constants.h256 /\ recallable x} =
-  createL_global Constants.h256_l
-let h384 : x:glbuffer uint64 8ul{witnessed x Constants.h384 /\ recallable x} =
-  createL_global Constants.h384_l
-let h512 : x:glbuffer uint64 8ul{witnessed x Constants.h512 /\ recallable x} =
-  createL_global Constants.h512_l
-
-
-noextract inline_for_extraction
-let index_h0 (a: sha2_alg) (i: size_t) : Stack (word a)
-  (requires (fun _ -> size_v i < 8))
-  (ensures (fun h0 r h1 ->
-    h0 == h1 /\
-    r == Seq.index (Spec.h0 a) (size_v i))) =
-    match a with
-    | SHA2_224 -> recall h224; recall_contents h224 Constants.h224; h224.(i)
-    | SHA2_256 -> recall h256; recall_contents h256 Constants.h256; h256.(i)
-    | SHA2_384 -> recall h384; recall_contents h384 Constants.h384; h384.(i)
-    | SHA2_512 -> recall h512; recall_contents h512 Constants.h512; h512.(i)
-
-
-let k224_256 : x:glbuffer uint32 64ul{witnessed x Constants.k224_256 /\ recallable x} =
-  createL_global Constants.k224_256_l
-
-let k384_512 : x:glbuffer uint64 80ul{witnessed x Constants.k384_512 /\ recallable x} =
-  createL_global Constants.k384_512_l
-
-
-noextract inline_for_extraction
-let index_k0 (a:sha2_alg) (i:size_t) : Stack (word a)
-  (requires (fun _ -> size_v i < Spec.size_k_w a))
-  (ensures (fun h0 r h1 ->
-    h0 == h1 /\
-    r == Seq.index (Spec.k0 a) (size_v i))) =
-  match a with
-  | SHA2_224 | SHA2_256 ->
-      recall_contents k224_256 Constants.k224_256;
-      k224_256.(i)
-  | SHA2_384 | SHA2_512 ->
-      recall_contents k384_512 Constants.k384_512;
-      k384_512.(i)
-
-
-unfold let block_t (a:sha2_alg) =
+unfold
+let block_t (a:sha2_alg) =
   lbuffer uint8 (block_len a)
 
-inline_for_extraction
+inline_for_extraction noextract
 let ws_t (a:sha2_alg) (m:m_spec) =
   lbuffer (element_t a m) 16ul
 
-inline_for_extraction
-val shuffle_core: #a: sha2_alg -> #m:m_spec ->
-  k_t: word a ->
-  ws_t: element_t a m ->
-  st: state_t a m ->
+
+inline_for_extraction noextract
+val set_wsi: #a:sha2_alg -> #m:m_spec
+  -> ws:ws_t a m
+  -> i:size_t{v i < 16}
+  -> b:lbuffer uint8 (block_len a)
+  -> bi:size_t{v bi < 16 / (lanes a m)} ->
   Stack unit
-    (requires (fun h -> live h st))
-    (ensures (fun h0 _ h1 ->
-      modifies (loc st) h0 h1 /\
-      as_seq h1 st ==
-      SpecVec.shuffle_core_spec k_t ws_t (as_seq h0 st)))
+  (requires fun h -> live h b /\ live h ws /\ disjoint b ws)
+  (ensures  fun h0 _ h1 -> modifies (loc ws) h0 h1 /\
+    as_seq h1 ws == LSeq.upd (as_seq h0 ws) (v i) (SpecVec.load_elementi #a #m (as_seq h0 b) (v bi)))
 
-#push-options "--z3rlimit 400"
-let shuffle_core #a #m k_t ws_t st =
-  let hp0 = ST.get() in
-  let a0 = st.(0ul) in
-  let b0 = st.(1ul) in
-  let c0 = st.(2ul) in
-  let d0 = st.(3ul) in
-  let e0 = st.(4ul) in
-  let f0 = st.(5ul) in
-  let g0 = st.(6ul) in
-  let h0 = st.(7ul) in
-  let k_e_t = load_element a m k_t in
-  let t1 = h0 +| (_Sigma1 e0) +| (_Ch e0 f0 g0) +| k_e_t +| ws_t in
-  let t2 = (_Sigma0 a0) +| (_Maj a0 b0 c0) in
-  let a1 = t1 +| t2 in
-  let b1 = a0 in
-  let c1 = b0 in
-  let d1 = c0 in
-  let e1 = d0 +| t1 in
-  let f1 = e0 in
-  let g1 = f0 in
-  let h1 = g0 in
-  st.(0ul) <- a1;
-  st.(1ul) <- b1;
-  st.(2ul) <- c1;
-  st.(3ul) <- d1;
-  st.(4ul) <- e1;
-  st.(5ul) <- f1;
-  st.(6ul) <- g1;
-  st.(7ul) <- h1;
-  let h1 = ST.get() in
-  LSeq.eq_intro (as_seq h1 st)
-           (shuffle_core_spec k_t ws_t (as_seq hp0 st))
-#pop-options
-
-inline_for_extraction
-val set_wsi (#a:sha2_alg) (#m:m_spec) (ws:ws_t a m) (i:size_t{v i < 16}) (b:lbuffer uint8 (block_len a)) (bi:size_t{v bi < 16 / (lanes a m)}):
-            Stack unit
-            (requires (fun h -> live h b /\ live h ws /\ disjoint b ws))
-            (ensures (fun h0 _ h1 -> modifies (loc ws) h0 h1 /\
-                                    as_seq h1 ws == LSeq.upd (as_seq h0 ws) (v i)
-                                                    (SpecVec.load_elementi #a #m (as_seq h0 b) (v bi))))
-#push-options "--z3rlimit 100"
 let set_wsi #a #m ws i b bi =
   [@inline_let]
   let l = lanes a m in
-  ws.(i) <- vec_load_be (word_t a) l (sub b (bi *. size l *. word_len a) (size l *. word_len a))
-#pop-options
+  ws.(i) <- vec_load_be (word_t a) l (sub b (bi *! size l *! word_len a) (size l *! word_len a))
+
 
 noextract
 let load_blocks_spec1 (#a:sha2_alg) (#m:m_spec{lanes a m == 1}) (b:multiblock_spec a m) : ws_spec a m =
@@ -165,18 +78,20 @@ let load_blocks_spec1 (#a:sha2_alg) (#m:m_spec{lanes a m == 1}) (b:multiblock_sp
 
 noextract
 let load_blocks_spec1_lemma (#a:sha2_alg) (#m:m_spec{lanes a m == 1}) (b:multiblock_spec a m) :
-  Lemma (SpecVec.load_blocks b == load_blocks_spec1 b) =
+  Lemma (SpecVec.load_blocks b == load_blocks_spec1 b)
+ =
   LSeq.eq_intro (SpecVec.load_blocks b) (load_blocks_spec1 b)
 
-inline_for_extraction
-val load_blocks1 (#a: sha2_alg) (#m:m_spec{lanes a m == 1})
-                 (b: multibuf (lanes a m) (block_len a)) (ws: ws_t a m):
-    Stack unit
-    (requires (fun h -> live_multi h b /\ live h ws /\ disjoint_multi b ws))
-    (ensures (fun h0 _ h1 -> modifies (loc ws) h0 h1 /\
-                           as_seq h1 ws ==
-                           SpecVec.load_blocks (as_seq_multi h0 b)))
-#push-options "--z3rlimit 100"
+
+inline_for_extraction noextract
+val load_blocks1: #a:sha2_alg -> #m:m_spec{lanes a m == 1}
+  -> b:multibuf (lanes a m) (block_len a)
+  -> ws:ws_t a m ->
+  Stack unit
+  (requires fun h -> live_multi h b /\ live h ws /\ disjoint_multi b ws)
+  (ensures  fun h0 _ h1 -> modifies (loc ws) h0 h1 /\
+    as_seq h1 ws == SpecVec.load_blocks (as_seq_multi h0 b))
+
 let load_blocks1 #a #m ib ws =
   let h0 = ST.get() in
   let b = ib.(|0|) in
@@ -204,7 +119,7 @@ let load_blocks1 #a #m ib ws =
   load_blocks_spec1_lemma #a #m (as_seq_multi h0 ib);
   assert (as_seq h1 ws == load_blocks_spec1 (as_seq_multi h0 ib));
   assert (as_seq h1 ws == SpecVec.load_blocks (as_seq_multi h0 ib))
-#pop-options
+
 
 noextract
 let load_blocks_spec4 (#a:sha2_alg) (#m:m_spec{lanes a m == 4}) (b:multiblock_spec a m) : ws_spec a m =
@@ -231,19 +146,23 @@ let load_blocks_spec4 (#a:sha2_alg) (#m:m_spec{lanes a m == 4}) (b:multiblock_sp
   create16 ws0 ws1 ws2 ws3 ws4 ws5 ws6 ws7
            ws8 ws9 ws10 ws11 ws12 ws13 ws14 ws15
 
+
 noextract
 let load_blocks_spec4_lemma (#a:sha2_alg) (#m:m_spec{lanes a m == 4}) (b:multiblock_spec a m) :
-  Lemma (SpecVec.load_blocks b == load_blocks_spec4 b) =
+  Lemma (SpecVec.load_blocks b == load_blocks_spec4 b)
+ =
   LSeq.eq_intro (SpecVec.load_blocks b) (load_blocks_spec4 b)
 
-inline_for_extraction
-val load_blocks4 (#a: sha2_alg) (#m:m_spec{lanes a m == 4})
-                 (b: multibuf (lanes a m) (block_len a)) (ws: ws_t a m):
-    Stack unit
-    (requires (fun h -> live_multi h b /\ live h ws /\ disjoint_multi b ws))
-    (ensures (fun h0 _ h1 -> modifies (loc ws) h0 h1 /\
-                           as_seq h1 ws ==
-                           SpecVec.load_blocks (as_seq_multi h0 b)))
+
+inline_for_extraction noextract
+val load_blocks4: #a:sha2_alg -> #m:m_spec{lanes a m == 4}
+  -> b:multibuf (lanes a m) (block_len a)
+  -> ws:ws_t a m ->
+  Stack unit
+  (requires fun h -> live_multi h b /\ live h ws /\ disjoint_multi b ws)
+  (ensures  fun h0 _ h1 -> modifies (loc ws) h0 h1 /\
+    as_seq h1 ws == SpecVec.load_blocks (as_seq_multi h0 b))
+
 #push-options "--z3rlimit 150"
 let load_blocks4 #a #m ib ws =
   let h0 = ST.get() in
@@ -275,6 +194,7 @@ let load_blocks4 #a #m ib ws =
   ()
 #pop-options
 
+
 noextract
 let load_blocks_spec8 (#a:sha2_alg) (#m:m_spec{lanes a m == 8}) (b:multiblock_spec a m) : ws_spec a m =
   let b0 = b.(|0|) in
@@ -304,19 +224,23 @@ let load_blocks_spec8 (#a:sha2_alg) (#m:m_spec{lanes a m == 8}) (b:multiblock_sp
   create16 ws0 ws1 ws2 ws3 ws4 ws5 ws6 ws7
            ws8 ws9 ws10 ws11 ws12 ws13 ws14 ws15
 
+
 noextract
 let load_blocks_spec8_lemma (#a:sha2_alg) (#m:m_spec{lanes a m == 8}) (b:multiblock_spec a m) :
-  Lemma (SpecVec.load_blocks b == load_blocks_spec8 b) =
+  Lemma (SpecVec.load_blocks b == load_blocks_spec8 b)
+ =
   LSeq.eq_intro (SpecVec.load_blocks b) (load_blocks_spec8 b)
 
-inline_for_extraction
-val load_blocks8 (#a: sha2_alg) (#m:m_spec{lanes a m == 8})
-                 (b: multibuf (lanes a m) (block_len a)) (ws: ws_t a m):
-    Stack unit
-    (requires (fun h -> live_multi h b /\ live h ws /\ disjoint_multi b ws))
-    (ensures (fun h0 _ h1 -> modifies (loc ws) h0 h1 /\
-                           as_seq h1 ws ==
-                           SpecVec.load_blocks (as_seq_multi h0 b)))
+
+inline_for_extraction noextract
+val load_blocks8: #a:sha2_alg -> #m:m_spec{lanes a m == 8}
+  -> b:multibuf (lanes a m) (block_len a)
+  -> ws:ws_t a m ->
+  Stack unit
+  (requires fun h -> live_multi h b /\ live h ws /\ disjoint_multi b ws)
+  (ensures  fun h0 _ h1 -> modifies (loc ws) h0 h1 /\
+    as_seq h1 ws == SpecVec.load_blocks (as_seq_multi h0 b))
+
 #push-options "--z3rlimit 150"
 let load_blocks8 #a #m ib ws =
   let h0 = ST.get() in
@@ -348,14 +272,15 @@ let load_blocks8 #a #m ib ws =
   ()
 #pop-options
 
-inline_for_extraction
-val load_blocks (#a: sha2_alg) (#m:m_spec)
-                (b: multibuf (lanes a m) (block_len a)) (ws: ws_t a m):
-    Stack unit
-    (requires (fun h -> live_multi h b /\ live h ws /\ disjoint_multi b ws))
-    (ensures (fun h0 _ h1 -> modifies (loc ws) h0 h1 /\
-                           as_seq h1 ws ==
-                           SpecVec.load_blocks (as_seq_multi h0 b)))
+
+inline_for_extraction noextract
+val load_blocks: #a:sha2_alg -> #m:m_spec
+  -> b:multibuf (lanes a m) (block_len a)
+  -> ws:ws_t a m ->
+  Stack unit
+  (requires fun h -> live_multi h b /\ live h ws /\ disjoint_multi b ws)
+  (ensures  fun h0 _ h1 -> modifies (loc ws) h0 h1 /\
+    as_seq h1 ws == SpecVec.load_blocks (as_seq_multi h0 b))
 
 let load_blocks #a #m b ws =
   match lanes a m with
@@ -365,79 +290,41 @@ let load_blocks #a #m b ws =
   | _ -> admit()
 
 
-inline_for_extraction
-val transpose_ws4 (#a: sha2_alg) (#m:m_spec{lanes a m == 4}) (ws: ws_t a m):
-    Stack unit
-    (requires (fun h -> live h ws))
-    (ensures (fun h0 _ h1 -> modifies (loc ws) h0 h1 /\
-                           as_seq h1 ws ==
-                           SpecVec.transpose_ws (as_seq h0 ws)))
+inline_for_extraction noextract
+val transpose_ws4: #a:sha2_alg -> #m:m_spec{lanes a m == 4} -> ws:ws_t a m ->
+  Stack unit
+  (requires fun h -> live h ws)
+  (ensures  fun h0 _ h1 -> modifies (loc ws) h0 h1 /\
+    as_seq h1 ws == SpecVec.transpose_ws (as_seq h0 ws))
 
 let transpose_ws4 #a #m ws =
-  let h0 = ST.get() in
   let (ws0,ws1,ws2,ws3) = VecTranspose.transpose4x4 (ws.(0ul),ws.(1ul),ws.(2ul),ws.(3ul)) in
   let (ws4,ws5,ws6,ws7) = VecTranspose.transpose4x4 (ws.(4ul),ws.(5ul),ws.(6ul),ws.(7ul)) in
   let (ws8,ws9,ws10,ws11) = VecTranspose.transpose4x4 (ws.(8ul),ws.(9ul),ws.(10ul),ws.(11ul)) in
   let (ws12,ws13,ws14,ws15) = VecTranspose.transpose4x4 (ws.(12ul),ws.(13ul),ws.(14ul),ws.(15ul)) in
-  ws.(0ul) <- ws0;
-  ws.(1ul) <- ws1;
-  ws.(2ul) <- ws2;
-  ws.(3ul) <- ws3;
-  ws.(4ul) <- ws4;
-  ws.(5ul) <- ws5;
-  ws.(6ul) <- ws6;
-  ws.(7ul) <- ws7;
-  ws.(8ul) <- ws8;
-  ws.(9ul) <- ws9;
-  ws.(10ul) <- ws10;
-  ws.(11ul) <- ws11;
-  ws.(12ul) <- ws12;
-  ws.(13ul) <- ws13;
-  ws.(14ul) <- ws14;
-  ws.(15ul) <- ws15;
-  let h1 = ST.get() in
-  LSeq.eq_intro (as_seq h1 ws) (SpecVec.transpose_ws (as_seq h0 ws))
+  create16_st ws ws0 ws1 ws2 ws3 ws4 ws5 ws6 ws7 ws8 ws9 ws10 ws11 ws12 ws13 ws14 ws15
 
-inline_for_extraction
-val transpose_ws8 (#a: sha2_alg) (#m:m_spec{lanes a m == 8}) (ws: ws_t a m):
-    Stack unit
-    (requires (fun h -> live h ws))
-    (ensures (fun h0 _ h1 -> modifies (loc ws) h0 h1 /\
-                           as_seq h1 ws ==
-                           SpecVec.transpose_ws (as_seq h0 ws)))
+
+inline_for_extraction noextract
+val transpose_ws8: #a:sha2_alg -> #m:m_spec{lanes a m == 8} -> ws:ws_t a m ->
+  Stack unit
+  (requires fun h -> live h ws)
+  (ensures  fun h0 _ h1 -> modifies (loc ws) h0 h1 /\
+    as_seq h1 ws == SpecVec.transpose_ws (as_seq h0 ws))
 
 let transpose_ws8 #a #m ws =
-  let h0 = ST.get() in
   let (ws0,ws1,ws2,ws3,ws4,ws5,ws6,ws7) = VecTranspose.transpose8x8 (ws.(0ul),ws.(1ul),ws.(2ul),ws.(3ul),ws.(4ul),ws.(5ul),ws.(6ul),ws.(7ul)) in
   let (ws8,ws9,ws10,ws11,ws12,ws13,ws14,ws15) = VecTranspose.transpose8x8 (ws.(8ul),ws.(9ul),ws.(10ul),ws.(11ul),ws.(12ul),ws.(13ul),ws.(14ul),ws.(15ul)) in
-  ws.(0ul) <- ws0;
-  ws.(1ul) <- ws1;
-  ws.(2ul) <- ws2;
-  ws.(3ul) <- ws3;
-  ws.(4ul) <- ws4;
-  ws.(5ul) <- ws5;
-  ws.(6ul) <- ws6;
-  ws.(7ul) <- ws7;
-  ws.(8ul) <- ws8;
-  ws.(9ul) <- ws9;
-  ws.(10ul) <- ws10;
-  ws.(11ul) <- ws11;
-  ws.(12ul) <- ws12;
-  ws.(13ul) <- ws13;
-  ws.(14ul) <- ws14;
-  ws.(15ul) <- ws15;
-  let h1 = ST.get() in
-  LSeq.eq_intro (as_seq h1 ws) (SpecVec.transpose_ws8 (as_seq h0 ws))
+  create16_st ws ws0 ws1 ws2 ws3 ws4 ws5 ws6 ws7 ws8 ws9 ws10 ws11 ws12 ws13 ws14 ws15
 
 
+inline_for_extraction noextract
+val transpose_ws: #a:sha2_alg -> #m:m_spec -> ws:ws_t a m ->
+  Stack unit
+  (requires fun h -> live h ws)
+  (ensures  fun h0 _ h1 -> modifies (loc ws) h0 h1 /\
+    as_seq h1 ws == SpecVec.transpose_ws (as_seq h0 ws))
 
-inline_for_extraction
-val transpose_ws (#a: sha2_alg) (#m:m_spec) (ws: ws_t a m):
-    Stack unit
-    (requires (fun h -> live h ws))
-    (ensures (fun h0 _ h1 -> modifies (loc ws) h0 h1 /\
-                           as_seq h1 ws ==
-                           SpecVec.transpose_ws (as_seq h0 ws)))
 let transpose_ws #a #m ws =
   match lanes a m with
   | 1 -> ()
@@ -446,144 +333,43 @@ let transpose_ws #a #m ws =
   | _ -> admit()
 
 
-inline_for_extraction
-val load_ws (#a: sha2_alg) (#m:m_spec)
-            (b: multibuf (lanes a m) (block_len a)) (ws: ws_t a m):
-    Stack unit
-    (requires (fun h ->
-      live_multi h b /\ live h ws /\ disjoint_multi b ws))
-    (ensures (fun h0 _ h1 ->
-      modifies (loc ws) h0 h1 /\
-      as_seq h1 ws == SpecVec.load_ws #a #m (as_seq_multi h0 b)))
+inline_for_extraction noextract
+val load_ws: #a:sha2_alg -> #m:m_spec
+  -> b:multibuf (lanes a m) (block_len a)
+  -> ws:ws_t a m ->
+  Stack unit
+  (requires fun h -> live_multi h b /\ live h ws /\ disjoint_multi b ws)
+  (ensures  fun h0 _ h1 -> modifies (loc ws) h0 h1 /\
+    as_seq h1 ws == SpecVec.load_ws #a #m (as_seq_multi h0 b))
+
 let load_ws #a #m b ws =
-    let h0 = ST.get() in
-    load_blocks b ws;
-    transpose_ws ws
-
-#push-options "--z3rlimit 300"
-inline_for_extraction
-val ws_next (#a: sha2_alg) (#m:m_spec)
-            (ws: ws_t a m):
-    Stack unit
-    (requires (fun h -> live h ws))
-    (ensures (fun h0 _ h1 ->
-      modifies (loc ws) h0 h1 /\
-      as_seq h1 ws == SpecVec.ws_next (as_seq h0 ws)))
-let ws_next #a #m ws =
-  let h0 = ST.get() in
-  loop1 h0 16ul ws
-    (fun h -> ws_next_inner #a #m)
-    (fun i ->
-      Lib.LoopCombinators.unfold_repeati 16 (ws_next_inner #a #m) (as_seq h0 ws) (v i);
-      let t16 = ws.(i) in
-      let t15 = ws.((i+.1ul) %. 16ul) in
-      let t7  = ws.((i+.9ul) %. 16ul) in
-      let t2  = ws.((i+.14ul) %. 16ul) in
-      let s1 = _sigma1 t2 in
-      let s0 = _sigma0 t15 in
-      ws.(i) <- (s1 +| t7 +| s0 +| t16))
-#pop-options
-
-inline_for_extraction
-val shuffle: #a:sha2_alg -> #m:m_spec -> ws:ws_t a m -> hash:state_t a m ->
-    Stack unit
-    (requires (fun h ->
-      live h hash /\ live h ws /\
-      disjoint hash ws))
-    (ensures (fun h0 _ h1 ->
-      modifies2 ws hash h0 h1 /\
-      as_seq h1 hash == SpecVec.shuffle #a #m (as_seq h0 ws) (as_seq h0 hash)))
-
-let shuffle #a #m ws hash =
-  let h0 = ST.get() in
-  loop2 h0 (num_rounds16 a) ws hash
-    (fun h -> shuffle_inner_loop #a #m)
-    (fun i ->
-      Lib.LoopCombinators.unfold_repeati (v (num_rounds16 a)) (shuffle_inner_loop #a #m) (as_seq h0 ws, as_seq h0 hash) (v i);
-      let h1 = ST.get() in
-      loop1 h1 16ul hash
-      (fun h -> shuffle_inner #a #m (as_seq h1 ws) (v i))
-      (fun j ->
-       Lib.LoopCombinators.unfold_repeati 16 (shuffle_inner #a #m (as_seq h1 ws) (v i)) (as_seq h1 hash) (v j);
-       let k_t = index_k0 a (16ul *. i +. j) in
-       let ws_t = ws.(j) in
-       shuffle_core k_t ws_t hash);
-      if i <. num_rounds16 a -. 1ul then
-        ws_next ws)
+  load_blocks b ws;
+  transpose_ws ws
 
 
-(** Init *)
-inline_for_extraction
-val alloc: a:sha2_alg -> m:m_spec ->
-    StackInline (state_t a m)
-    (requires (fun h -> True))
-    (ensures (fun h0 b h1 -> live h1 b /\ stack_allocated b h0 h1 (Seq.create 8 (zero_element a m))))
-let alloc a m = Lib.Buffer.create 8ul (zero_element a m)
-
-let init #a #m hash =
-  let h0 = ST.get() in
-  fill h0 8ul hash
-  (fun h i -> load_element a m (Seq.index (Spec.h0 a) i))
-  (fun i -> let hi = index_h0 a i in
-          load_element a m hi);
-  let h1 = ST.get() in
-  LSeq.eq_intro (as_seq h1 hash)
-           (LSeq.createi 8 (fun i -> load_element a m (Seq.index (Spec.h0 a) i)))
-
-#push-options "--z3rlimit 200"
-let update #a #m b hash =
-  let h0 = ST.get() in
-  push_frame ();
-  let h1 = ST.get() in
-  let hash_old = create 8ul (zero_element a m) in
-  let ws = create 16ul (zero_element a m) in
-  assert (disjoint_multi b hash_old);
-  assert (disjoint_multi b ws);
-  assert (disjoint ws hash_old);
-  assert (disjoint hash hash_old);
-  assert (disjoint ws hash);
-  copy hash_old hash;
-  let h2 = ST.get() in
-  assert (live_multi h2 b);
-  Lib.NTuple.(eq_intro (as_seq_multi h2 b) (as_seq_multi h0 b));
-  load_ws b ws;
-  let h3 = ST.get() in
-  assert (modifies (loc ws |+| loc hash_old) h0 h3);
-  assert (as_seq h3 ws == Hacl.Spec.SHA2.Vec.load_ws (as_seq_multi h2 b));
-  shuffle ws hash;
-  let h4 = ST.get() in
-  assert (modifies (loc hash |+| (loc ws |+| loc hash_old)) h0 h4);
-  assert (as_seq h4 hash == Hacl.Spec.SHA2.Vec.shuffle (as_seq h3 ws) (as_seq h0 hash));
-  map2T 8ul hash (+|) hash hash_old;
-  let h5 = ST.get() in
-  assert (modifies (loc hash |+| (loc ws |+| loc hash_old)) h0 h5);
-  reveal_opaque (`%SpecVec.update) (SpecVec.update #a #m);
-  assert (as_seq h5 hash == SpecVec.update (as_seq_multi h0 b) (as_seq h0 hash));
-  pop_frame()
-#pop-options
-
-inline_for_extraction
+inline_for_extraction noextract
 let padded_blocks (a:sha2_alg) (len:size_t{v len < block_length a}) :
-                  n:size_t{v n == SpecVec.padded_blocks a (v len)} =
-  if (len +. len_len a +. 1ul <=. block_len a) then 1ul else 2ul
+  n:size_t{v n == SpecVec.padded_blocks a (v len)}
+ =
+  if (len +! len_len a +! 1ul <=. block_len a) then 1ul else 2ul
 
 
-inline_for_extraction
-val load_last_blocks: #a:sha2_alg ->
-                      totlen_buf:lbuffer uint8 (len_len a) ->
-                      len:size_t{v len < block_length a} ->
-                      b:lbuffer uint8 len ->
-                      fin:size_t{v fin == block_length a \/ v fin == 2 * block_length a} ->
-                      last:lbuffer uint8 (2ul *. block_len a) ->
-    Stack (lbuffer uint8 (block_len a) & lbuffer uint8 (block_len a))
-    (requires (fun h -> live h totlen_buf /\ live h b /\ live h last /\
-                      disjoint b last /\ disjoint last totlen_buf /\
-                      as_seq h last == LSeq.create (2 * block_length a) (u8 0)))
-    (ensures (fun h0 (l0,l1) h1 -> modifies (loc last) h0 h1 /\
-                           live h1 l0 /\ live h1 l1 /\
-                           (forall a l (r:lbuffer a l). disjoint last r ==> (disjoint l0 r /\ disjoint l1 r)) /\
-                           (as_seq h1 l0, as_seq h1 l1) ==
-                           SpecVec.load_last_blocks #a (as_seq h0 totlen_buf) (v fin) (v len) (as_seq h0 b)))
+inline_for_extraction noextract
+val load_last_blocks: #a:sha2_alg
+  -> totlen_buf:lbuffer uint8 (len_len a)
+  -> len:size_t{v len < block_length a}
+  -> b:lbuffer uint8 len
+  -> fin:size_t{v fin == block_length a \/ v fin == 2 * block_length a}
+  -> last:lbuffer uint8 (2ul *! block_len a)  ->
+  Stack (lbuffer uint8 (block_len a) & lbuffer uint8 (block_len a))
+  (requires fun h -> live h totlen_buf /\ live h b /\ live h last /\
+    disjoint b last /\ disjoint last totlen_buf /\
+    as_seq h last == LSeq.create (2 * block_length a) (u8 0))
+  (ensures (fun h0 (l0,l1) h1 -> modifies (loc last) h0 h1 /\
+    live h1 l0 /\ live h1 l1 /\
+    (forall a l (r:lbuffer a l). disjoint last r ==> (disjoint l0 r /\ disjoint l1 r)) /\
+    (as_seq h1 l0, as_seq h1 l1) == SpecVec.load_last_blocks #a (as_seq h0 totlen_buf) (v fin) (v len) (as_seq h0 b)))
+
 #push-options "--z3rlimit 200"
 let load_last_blocks #a totlen_buf len b fin last =
   let h0 = ST.get() in
@@ -597,28 +383,34 @@ let load_last_blocks #a totlen_buf len b fin last =
   (last0,last1)
 #pop-options
 
+
 noextract
 let preserves_sub_disjoint_multi #lanes #len #len' (b:lbuffer uint8 len) (r:multibuf lanes len') =
     (forall a l (x:lbuffer a l). disjoint b x ==> disjoint_multi r x)
 
+
+inline_for_extraction noextract
 let load_last_t (a:sha2_alg) (m:m_spec) =
-                  totlen_buf:lbuffer uint8 (len_len a) ->
-                  len:size_t{v len < block_length a} ->
-                  b:multibuf (lanes a m) len ->
-                  fin:size_t{v fin == block_length a \/ v fin == 2 * block_length a} ->
-                  last:lbuffer uint8 (size (lanes a m) *. 2ul *. block_len a) ->
-    Stack (multibuf (lanes a m) (block_len a) & multibuf (lanes a m) (block_len a))
-      (requires (fun h -> live h totlen_buf /\ live_multi h b /\ live h last /\
-                      disjoint_multi b last /\ disjoint last totlen_buf /\
-                      as_seq h last == LSeq.create (lanes a m * 2 * block_length a) (u8 0)))
-      (ensures (fun h0 (l0,l1) h1 -> modifies (loc last) h0 h1 /\
-                           live_multi h1 l0 /\ live_multi h1 l1 /\
-                           preserves_sub_disjoint_multi last l0 /\
-                           preserves_sub_disjoint_multi last l1 /\
-                           (as_seq_multi h1 l0, as_seq_multi h1 l1) ==
-                           SpecVec.load_last #a #m (as_seq h0 totlen_buf) (v fin) (v len) (as_seq_multi h0 b)))
-inline_for_extraction
+    totlen_buf:lbuffer uint8 (len_len a)
+  -> len:size_t{v len < block_length a}
+  -> b:multibuf (lanes a m) len
+  -> fin:size_t{v fin == block_length a \/ v fin == 2 * block_length a}
+  -> last:lbuffer uint8 (size (lanes a m) *! 2ul *! block_len a) ->
+  Stack (multibuf (lanes a m) (block_len a) & multibuf (lanes a m) (block_len a))
+  (requires  fun h -> live h totlen_buf /\ live_multi h b /\ live h last /\
+    disjoint_multi b last /\ disjoint last totlen_buf /\
+    as_seq h last == LSeq.create (lanes a m * 2 * block_length a) (u8 0))
+  (ensures  fun h0 (l0,l1) h1 -> modifies (loc last) h0 h1 /\
+    live_multi h1 l0 /\ live_multi h1 l1 /\
+    preserves_sub_disjoint_multi last l0 /\
+    preserves_sub_disjoint_multi last l1 /\
+    (as_seq_multi h1 l0, as_seq_multi h1 l1) ==
+    SpecVec.load_last #a #m (as_seq h0 totlen_buf) (v fin) (v len) (as_seq_multi h0 b))
+
+
+inline_for_extraction noextract
 val load_last1: #a:sha2_alg -> #m:m_spec{lanes a m = 1} -> load_last_t a m
+
 #push-options "--z3rlimit 250"
 let load_last1 #a #m totlen_buf len b fin last =
   let h0 = ST.get() in
@@ -638,16 +430,16 @@ let load_last1 #a #m totlen_buf len b fin last =
 #pop-options
 
 
-inline_for_extraction
+inline_for_extraction noextract
 val load_last4: #a:sha2_alg -> #m:m_spec{lanes a m = 4} -> load_last_t a m
 #push-options "--z3rlimit 350"
 let load_last4 #a #m totlen_buf len b fin last =
   let h0 = ST.get() in
   let (b0,(b1,(b2,b3))) = NTup.tup4 b in
-  let last0 = sub last 0ul (2ul *. block_len a) in
-  let last1 = sub last (2ul *. block_len a) (2ul *. block_len a) in
-  let last2 = sub last (4ul *. block_len a) (2ul *. block_len a) in
-  let last3 = sub last (6ul *. block_len a) (2ul *. block_len a) in
+  let last0 = sub last 0ul (2ul *! block_len a) in
+  let last1 = sub last (2ul *! block_len a) (2ul *! block_len a) in
+  let last2 = sub last (4ul *! block_len a) (2ul *! block_len a) in
+  let last3 = sub last (6ul *! block_len a) (2ul *! block_len a) in
   let h1 = ST.get() in
   assert (disjoint last0 last1);
   LSeq.eq_intro (as_seq h1 last0) (LSeq.create (2 * block_length a) (u8 0));
@@ -679,20 +471,21 @@ let load_last4 #a #m totlen_buf len b fin last =
   (mb0, mb1)
 #pop-options
 
-inline_for_extraction
+
+inline_for_extraction noextract
 val load_last8: #a:sha2_alg -> #m:m_spec{lanes a m = 8} -> load_last_t a m
 #push-options "--z3rlimit 600"
 let load_last8 #a #m totlen_buf len b fin last =
   let h0 = ST.get() in
   let (b0,(b1,(b2,(b3,(b4,(b5,(b6,b7))))))) = NTup.tup8 b in
-  let last0 = sub last 0ul (2ul *. block_len a) in
-  let last1 = sub last (2ul *. block_len a) (2ul *. block_len a) in
-  let last2 = sub last (4ul *. block_len a) (2ul *. block_len a) in
-  let last3 = sub last (6ul *. block_len a) (2ul *. block_len a) in
-  let last4 = sub last (8ul *. block_len a) (2ul *. block_len a) in
-  let last5 = sub last (10ul *. block_len a) (2ul *. block_len a) in
-  let last6 = sub last (12ul *. block_len a) (2ul *. block_len a) in
-  let last7 = sub last (14ul *. block_len a) (2ul *. block_len a) in
+  let last0 = sub last 0ul (2ul *! block_len a) in
+  let last1 = sub last (2ul *! block_len a) (2ul *! block_len a) in
+  let last2 = sub last (4ul *! block_len a) (2ul *! block_len a) in
+  let last3 = sub last (6ul *! block_len a) (2ul *! block_len a) in
+  let last4 = sub last (8ul *! block_len a) (2ul *! block_len a) in
+  let last5 = sub last (10ul *! block_len a) (2ul *! block_len a) in
+  let last6 = sub last (12ul *! block_len a) (2ul *! block_len a) in
+  let last7 = sub last (14ul *! block_len a) (2ul *! block_len a) in
   assert (internally_disjoint8 last0 last1 last2 last3 last4 last5 last6 last7);
   let h1 = ST.get() in
   assert (h0 == h1);
@@ -737,7 +530,8 @@ let load_last8 #a #m totlen_buf len b fin last =
   (mb0, mb1)
 #pop-options
 
-inline_for_extraction
+
+inline_for_extraction noextract
 val load_last: #a:sha2_alg -> #m:m_spec -> load_last_t a m
 let load_last #a #m  totlen_buf len b fin last =
   match lanes a m with
@@ -746,128 +540,39 @@ let load_last #a #m  totlen_buf len b fin last =
   | 8 -> load_last8 #a #m totlen_buf len b fin last
   | _ -> admit()
 
-#push-options "--z3rlimit 350"
-let update_last #a #m upd totlen len b hash =
-  let h0 = ST.get() in
-  push_frame ();
-  let h1 = ST.get() in
-  let blocks = padded_blocks a len in
-  let fin = blocks *. block_len a in
-  let last = create (size (lanes a m) *. 2ul *. block_len a) (u8 0) in
-  let totlen_buf = create (len_len a) (u8 0) in
-  let total_len_bits = secret (shift_left #(len_int_type a) totlen 3ul) in
-  Lib.ByteBuffer.uint_to_bytes_be #(len_int_type a) totlen_buf total_len_bits;
-  let h2 = ST.get () in
-  NTup.eq_intro (as_seq_multi h2 b) (as_seq_multi h0 b);
-  assert (as_seq h2 totlen_buf ==
-          Lib.ByteSequence.uint_to_bytes_be #(len_int_type a) total_len_bits);
-  let (last0,last1) = load_last #a #m totlen_buf len b fin last in
-  let h3 = ST.get () in
-  assert ((as_seq_multi h3 last0, as_seq_multi h3 last1) ==
-          SpecVec.load_last #a #m (as_seq h2 totlen_buf) (v fin) (v len) (as_seq_multi h2 b));
-  assert (disjoint_multi last1 hash);
-  upd last0 hash;
-  let h4 = ST.get() in
-  assert (modifies (loc hash |+| loc last |+| loc totlen_buf) h1 h3);
-  assert (as_seq h4 hash == SpecVec.update (as_seq_multi h3 last0) (as_seq h3 hash));
-  NTup.eq_intro (as_seq_multi h4 last1) (as_seq_multi h3 last1);
-  assert (v blocks > 1 ==> blocks >. 1ul);
-  assert (blocks >. 1ul ==> v blocks > 1);
-  assert (not (blocks >. 1ul) ==> not (v blocks > 1));
-  if blocks >. 1ul then (
-    upd last1 hash;
-    let h5 = ST.get() in
-    assert (as_seq h5 hash == SpecVec.update (as_seq_multi h4 last1) (as_seq h4 hash));
-    assert (modifies (loc hash |+| loc last |+| loc totlen_buf) h1 h5);
-    assert (as_seq h5 hash == SpecVec.update_last totlen (v len) (as_seq_multi h0 b) (as_seq h0 hash));
-    pop_frame()
-  ) else (
-    let h6 = ST.get() in
-    assert (h4 == h6);
-    assert (modifies (loc hash |+| loc totlen_buf |+| loc last) h1 h6);
-    assert (as_seq h6 hash == SpecVec.update_last totlen (v len) (as_seq_multi h0 b) (as_seq h0 hash));
-    pop_frame())
-#pop-options
 
-inline_for_extraction
-val transpose_state4 (#a: sha2_alg) (#m:m_spec{lanes a m == 4}) (st: state_t a m):
-    Stack unit
-    (requires (fun h -> live h st))
-    (ensures (fun h0 _ h1 -> modifies (loc st) h0 h1 /\
-                           as_seq h1 st ==
-                           SpecVec.transpose_state4 (as_seq h0 st)))
+inline_for_extraction noextract
+val transpose_state4: #a:sha2_alg -> #m:m_spec{lanes a m == 4} -> st:state_t a m ->
+  Stack unit
+  (requires fun h -> live h st)
+  (ensures  fun h0 _ h1 -> modifies (loc st) h0 h1 /\
+    as_seq h1 st == SpecVec.transpose_state4 (as_seq h0 st))
 
-#push-options "--z3rlimit 200"
 let transpose_state4 #a #m st =
-  let h0 = ST.get() in
-  let st0 = st.(0ul) in
-  let st1 = st.(1ul) in
-  let st2 = st.(2ul) in
-  let st3 = st.(3ul) in
-  let st4 = st.(4ul) in
-  let st5 = st.(5ul) in
-  let st6 = st.(6ul) in
-  let st7 = st.(7ul) in
-  let (st0',st1',st2',st3') = VecTranspose.transpose4x4 (st0,st1,st2,st3) in
-  let (st4',st5',st6',st7') = VecTranspose.transpose4x4 (st4,st5,st6,st7) in
-  st.(0ul) <- st0';
-  st.(1ul) <- st4';
-  st.(2ul) <- st1';
-  st.(3ul) <- st5';
-  st.(4ul) <- st2';
-  st.(5ul) <- st6';
-  st.(6ul) <- st3';
-  st.(7ul) <- st7';
-  let h1 = ST.get() in
-  LSeq.eq_intro (as_seq h1 st) (create8 st0' st4' st1' st5' st2' st6' st3' st7');
-  LSeq.eq_intro (as_seq h0 st) (create8 st0 st1 st2 st3 st4 st5 st6 st7);
-  LSeq.eq_intro (create8 st0' st4' st1' st5' st2' st6' st3' st7')
-                        (SpecVec.transpose_state4 (create8 st0 st1 st2 st3 st4 st5 st6 st7));
-  ()
+  let (st0',st1',st2',st3') = VecTranspose.transpose4x4 (st.(0ul),st.(1ul),st.(2ul),st.(3ul)) in
+  let (st4',st5',st6',st7') = VecTranspose.transpose4x4 (st.(4ul),st.(5ul),st.(6ul),st.(7ul)) in
+  create8_st st st0' st4' st1' st5' st2' st6' st3' st7'
 
 
-inline_for_extraction
-val transpose_state8 (#a: sha2_alg) (#m:m_spec{lanes a m == 8}) (st: state_t a m):
-    Stack unit
-    (requires (fun h -> live h st))
-    (ensures (fun h0 _ h1 -> modifies (loc st) h0 h1 /\
-                           as_seq h1 st ==
-                           SpecVec.transpose_state8 (as_seq h0 st)))
+inline_for_extraction noextract
+val transpose_state8: #a:sha2_alg -> #m:m_spec{lanes a m == 8} -> st:state_t a m ->
+  Stack unit
+  (requires fun h -> live h st)
+  (ensures  fun h0 _ h1 -> modifies (loc st) h0 h1 /\
+    as_seq h1 st == SpecVec.transpose_state8 (as_seq h0 st))
+
 let transpose_state8 #a #m st =
-  let h0 = ST.get() in
-  let st0 = st.(0ul) in
-  let st1 = st.(1ul) in
-  let st2 = st.(2ul) in
-  let st3 = st.(3ul) in
-  let st4 = st.(4ul) in
-  let st5 = st.(5ul) in
-  let st6 = st.(6ul) in
-  let st7 = st.(7ul) in
-  let (st0',st1',st2',st3',st4',st5',st6',st7') = VecTranspose.transpose8x8 (st0,st1,st2,st3,st4,st5,st6,st7) in
-  st.(0ul) <- st0';
-  st.(1ul) <- st1';
-  st.(2ul) <- st2';
-  st.(3ul) <- st3';
-  st.(4ul) <- st4';
-  st.(5ul) <- st5';
-  st.(6ul) <- st6';
-  st.(7ul) <- st7';
-  let h1 = ST.get() in
-  LSeq.eq_intro (as_seq h1 st) (create8 st0' st1' st2' st3' st4' st5' st6' st7');
-  LSeq.eq_intro (as_seq h0 st) (create8 st0 st1 st2 st3 st4 st5 st6 st7);
-  LSeq.eq_intro (create8 st0' st1' st2' st3' st4' st5' st6' st7')
-                        (SpecVec.transpose_state8 (create8 st0 st1 st2 st3 st4 st5 st6 st7));
-  ()
-#pop-options
+  let (st0',st1',st2',st3',st4',st5',st6',st7') = VecTranspose.transpose8x8 (st.(0ul),st.(1ul),st.(2ul),st.(3ul),st.(4ul),st.(5ul),st.(6ul),st.(7ul)) in
+  create8_st st st0' st1' st2' st3' st4' st5' st6' st7'
 
 
-inline_for_extraction
-val transpose_state (#a: sha2_alg) (#m:m_spec) (st: state_t a m):
-    Stack unit
-    (requires (fun h -> live h st))
-    (ensures (fun h0 _ h1 -> modifies (loc st) h0 h1 /\
-                           as_seq h1 st ==
-                           SpecVec.transpose_state (as_seq h0 st)))
+inline_for_extraction noextract
+val transpose_state: #a:sha2_alg -> #m:m_spec -> st:state_t a m ->
+  Stack unit
+  (requires fun h -> live h st)
+  (ensures  fun h0 _ h1 -> modifies (loc st) h0 h1 /\
+    as_seq h1 st == SpecVec.transpose_state (as_seq h0 st))
+
 let transpose_state #a #m st =
   match lanes a m with
   | 1 -> ()
@@ -876,47 +581,46 @@ let transpose_state #a #m st =
   | _ -> admit()
 
 
-inline_for_extraction
-val store_state: #a:sha2_alg -> #m:m_spec->
-                 st:state_t a m ->
-                 hbuf:lbuffer uint8 (size (lanes a m) *. 8ul *. word_len a) ->
-    Stack unit
-    (requires (fun h -> live h hbuf /\ live h st /\ disjoint hbuf st /\
-                      as_seq h hbuf == LSeq.create (lanes a m * 8 * word_length a) (u8 0)))
-    (ensures (fun h0 _ h1 -> modifies (loc st |+| loc hbuf) h0 h1 /\
-                           as_seq h1 hbuf ==
-                           SpecVec.store_state #a #m (as_seq h0 st)))
+inline_for_extraction noextract
+val store_state: #a:sha2_alg -> #m:m_spec
+  -> st:state_t a m
+  -> hbuf:lbuffer uint8 (size (lanes a m) *! 8ul *! word_len a) ->
+  Stack unit
+  (requires fun h -> live h hbuf /\ live h st /\ disjoint hbuf st /\
+    as_seq h hbuf == LSeq.create (lanes a m * 8 * word_length a) (u8 0))
+  (ensures  fun h0 _ h1 -> modifies (loc st |+| loc hbuf) h0 h1 /\
+    as_seq h1 hbuf == SpecVec.store_state #a #m (as_seq h0 st))
+
 let store_state #a #m st hbuf =
   transpose_state st;
   Lib.IntVector.Serialize.vecs_store_be hbuf st
 
 
 noextract
-let emit1_spec (#a:sha2_alg) (#m:m_spec{lanes a m == 1})
-          (hseq:LSeq.lseq uint8 (lanes a m * 8 * word_length a)):
-          multiseq (lanes a m) (hash_length a) =
-    let hsub = LSeq.sub hseq 0 (hash_length a) in
-    ntup1 hsub
+let emit1_spec (#a:sha2_alg) (#m:m_spec{lanes a m == 1}) (hseq:LSeq.lseq uint8 (lanes a m * 8 * word_length a)) :
+  multiseq (lanes a m) (hash_length a)
+ =
+  let hsub = LSeq.sub hseq 0 (hash_length a) in
+  ntup1 hsub
 
 
 noextract
-let emit1_lemma (#a:sha2_alg) (#m:m_spec{lanes a m == 1})
-                (hseq:LSeq.lseq uint8 (lanes a m * 8 * word_length a)):
-                Lemma (emit1_spec #a #m hseq ==
-                       SpecVec.emit #a #m hseq) =
-    Lib.NTuple.eq_intro (emit1_spec #a #m hseq) (SpecVec.emit #a #m hseq)
+let emit1_lemma (#a:sha2_alg) (#m:m_spec{lanes a m == 1}) (hseq:LSeq.lseq uint8 (lanes a m * 8 * word_length a)) :
+  Lemma (emit1_spec #a #m hseq == SpecVec.emit #a #m hseq)
+ =
+  Lib.NTuple.eq_intro (emit1_spec #a #m hseq) (SpecVec.emit #a #m hseq)
 
 
-inline_for_extraction
-val emit1: #a:sha2_alg -> #m:m_spec{lanes a m = 1} ->
-             hbuf: lbuffer uint8 (8ul *. word_len a) ->
-             result:multibuf (lanes a m) (hash_len a) ->
-    Stack unit
-    (requires (fun h -> live_multi h result /\ live h hbuf /\
-                      internally_disjoint result /\ disjoint_multi result hbuf))
-    (ensures (fun h0 _ h1 -> modifies_multi result h0 h1 /\
-                           as_seq_multi h1 result ==
-                           SpecVec.emit #a #m (as_seq h0 hbuf)))
+inline_for_extraction noextract
+val emit1: #a:sha2_alg -> #m:m_spec{lanes a m = 1}
+  -> hbuf:lbuffer uint8 (8ul *! word_len a)
+  -> result:multibuf (lanes a m) (hash_len a) ->
+  Stack unit
+  (requires fun h -> live_multi h result /\ live h hbuf /\
+    internally_disjoint result /\ disjoint_multi result hbuf)
+  (ensures  fun h0 _ h1 -> modifies_multi result h0 h1 /\
+    as_seq_multi h1 result == SpecVec.emit #a #m (as_seq h0 hbuf))
+
 let emit1 #a #m hbuf result =
   let h0 = ST.get() in
   copy result.(|0|) (sub hbuf 0ul (hash_len a));
@@ -927,34 +631,35 @@ let emit1 #a #m hbuf result =
 
 
 noextract
-let emit4_spec (#a:sha2_alg) (#m:m_spec{lanes a m == 4})
-          (hseq:LSeq.lseq uint8 (lanes a m * 8 * word_length a)):
-          multiseq (lanes a m) (hash_length a) =
-    let open Lib.Sequence in
-    let h0 = sub hseq 0 (hash_length a) in
-    let h1 = sub hseq (8 * word_length a) (hash_length a) in
-    let h2 = sub hseq (16 * word_length a) (hash_length a) in
-    let h3 = sub hseq (24 * word_length a) (hash_length a) in
-    let hsub : multiseq 4 (hash_length a) = ntup4 (h0,(h1,(h2,h3))) in
-    hsub
+let emit4_spec (#a:sha2_alg) (#m:m_spec{lanes a m == 4}) (hseq:LSeq.lseq uint8 (lanes a m * 8 * word_length a)) :
+  multiseq (lanes a m) (hash_length a)
+ =
+  let open Lib.Sequence in
+  let h0 = sub hseq 0 (hash_length a) in
+  let h1 = sub hseq (8 * word_length a) (hash_length a) in
+  let h2 = sub hseq (16 * word_length a) (hash_length a) in
+  let h3 = sub hseq (24 * word_length a) (hash_length a) in
+  let hsub : multiseq 4 (hash_length a) = ntup4 (h0,(h1,(h2,h3))) in
+  hsub
+
 
 noextract
-let emit4_lemma (#a:sha2_alg) (#m:m_spec{lanes a m == 4})
-                (hseq:LSeq.lseq uint8 (lanes a m * 8 * word_length a)):
-                Lemma (emit4_spec #a #m hseq ==
-                       SpecVec.emit #a #m hseq) =
-    Lib.NTuple.eq_intro (emit4_spec #a #m hseq) (SpecVec.emit #a #m hseq)
+let emit4_lemma (#a:sha2_alg) (#m:m_spec{lanes a m == 4}) (hseq:LSeq.lseq uint8 (lanes a m * 8 * word_length a)) :
+  Lemma (emit4_spec #a #m hseq == SpecVec.emit #a #m hseq)
+ =
+  Lib.NTuple.eq_intro (emit4_spec #a #m hseq) (SpecVec.emit #a #m hseq)
 
-inline_for_extraction
-val emit4: #a:sha2_alg -> #m:m_spec{lanes a m = 4} ->
-             hbuf: lbuffer uint8 (size (lanes a m) *. 8ul *. word_len a) ->
-             result:multibuf (lanes a m) (hash_len a) ->
-    Stack unit
-    (requires (fun h -> live_multi h result /\ live h hbuf /\
-                      internally_disjoint result  /\ disjoint_multi result hbuf))
-    (ensures (fun h0 _ h1 -> modifies_multi result h0 h1 /\
-                           as_seq_multi h1 result ==
-                           SpecVec.emit #a #m (as_seq h0 hbuf)))
+
+inline_for_extraction noextract
+val emit4: #a:sha2_alg -> #m:m_spec{lanes a m = 4}
+  -> hbuf: lbuffer uint8 (size (lanes a m) *! 8ul *! word_len a)
+  -> result:multibuf (lanes a m) (hash_len a) ->
+  Stack unit
+  (requires fun h -> live_multi h result /\ live h hbuf /\
+    internally_disjoint result  /\ disjoint_multi result hbuf)
+  (ensures  fun h0 _ h1 -> modifies_multi result h0 h1 /\
+    as_seq_multi h1 result == SpecVec.emit #a #m (as_seq h0 hbuf))
+
 #push-options "--z3rlimit 200"
 let emit4 #a #m hbuf result =
   let h0 = ST.get() in
@@ -966,9 +671,9 @@ let emit4 #a #m hbuf result =
   assert (disjoint b1 b3);
   assert (disjoint b2 b3);
   copy b0 (sub hbuf 0ul (hash_len a));
-  copy b1 (sub hbuf (8ul *. word_len a) (hash_len a));
-  copy b2 (sub hbuf (16ul *. word_len a) (hash_len a));
-  copy b3 (sub hbuf (24ul *. word_len a) (hash_len a));
+  copy b1 (sub hbuf (8ul *! word_len a) (hash_len a));
+  copy b2 (sub hbuf (16ul *! word_len a) (hash_len a));
+  copy b3 (sub hbuf (24ul *! word_len a) (hash_len a));
   let h1 = ST.get() in
   assert (as_seq h1 b0 == LSeq.sub (as_seq h0 hbuf) 0 (hash_length a));
   assert (as_seq h1 b1 == LSeq.sub (as_seq h0 hbuf) (8 * word_length a) (hash_length a));
@@ -983,54 +688,56 @@ let emit4 #a #m hbuf result =
   ()
 #pop-options
 
-noextract
-let emit8_spec (#a:sha2_alg) (#m:m_spec{lanes a m == 8})
-          (hseq:LSeq.lseq uint8 (lanes a m * 8 * word_length a)):
-          multiseq (lanes a m) (hash_length a) =
-    let open Lib.Sequence in
-    let h0 = sub hseq 0 (hash_length a) in
-    let h1 = sub hseq (8 * word_length a) (hash_length a) in
-    let h2 = sub hseq (16 * word_length a) (hash_length a) in
-    let h3 = sub hseq (24 * word_length a) (hash_length a) in
-    let h4 = sub hseq (32 * word_length a) (hash_length a) in
-    let h5 = sub hseq (40 * word_length a) (hash_length a) in
-    let h6 = sub hseq (48 * word_length a) (hash_length a) in
-    let h7 = sub hseq (56 * word_length a) (hash_length a) in
-    let hsub : multiseq 8 (hash_length a) = ntup8 (h0,(h1,(h2,(h3,(h4,(h5,(h6,h7))))))) in
-    hsub
 
 noextract
-let emit8_lemma (#a:sha2_alg) (#m:m_spec{lanes a m == 8})
-                (hseq:LSeq.lseq uint8 (lanes a m * 8 * word_length a)):
-                Lemma (emit8_spec #a #m hseq ==
-                       SpecVec.emit #a #m hseq) =
-    Lib.NTuple.eq_intro (emit8_spec #a #m hseq) (SpecVec.emit #a #m hseq)
+let emit8_spec (#a:sha2_alg) (#m:m_spec{lanes a m == 8}) (hseq:LSeq.lseq uint8 (lanes a m * 8 * word_length a)) :
+  multiseq (lanes a m) (hash_length a)
+ =
+  let open Lib.Sequence in
+  let h0 = sub hseq 0 (hash_length a) in
+  let h1 = sub hseq (8 * word_length a) (hash_length a) in
+  let h2 = sub hseq (16 * word_length a) (hash_length a) in
+  let h3 = sub hseq (24 * word_length a) (hash_length a) in
+  let h4 = sub hseq (32 * word_length a) (hash_length a) in
+  let h5 = sub hseq (40 * word_length a) (hash_length a) in
+  let h6 = sub hseq (48 * word_length a) (hash_length a) in
+  let h7 = sub hseq (56 * word_length a) (hash_length a) in
+  let hsub : multiseq 8 (hash_length a) = ntup8 (h0,(h1,(h2,(h3,(h4,(h5,(h6,h7))))))) in
+  hsub
 
-inline_for_extraction
-val emit8: #a:sha2_alg -> #m:m_spec{lanes a m = 8} ->
-             hbuf: lbuffer uint8 (size (lanes a m) *. 8ul *. word_len a) ->
-             result:multibuf (lanes a m) (hash_len a) ->
-    Stack unit
-    (requires (fun h -> live_multi h result /\ live h hbuf /\
-                      internally_disjoint result  /\ disjoint_multi result hbuf))
-    (ensures (fun h0 _ h1 -> modifies_multi result h0 h1 /\
-                           as_seq_multi h1 result ==
-                           SpecVec.emit #a #m (as_seq h0 hbuf)))
+
+noextract
+let emit8_lemma (#a:sha2_alg) (#m:m_spec{lanes a m == 8}) (hseq:LSeq.lseq uint8 (lanes a m * 8 * word_length a)) :
+  Lemma (emit8_spec #a #m hseq == SpecVec.emit #a #m hseq)
+ =
+  Lib.NTuple.eq_intro (emit8_spec #a #m hseq) (SpecVec.emit #a #m hseq)
+
+
+inline_for_extraction noextract
+val emit8: #a:sha2_alg -> #m:m_spec{lanes a m = 8}
+  -> hbuf: lbuffer uint8 (size (lanes a m) *! 8ul *! word_len a)
+  -> result:multibuf (lanes a m) (hash_len a) ->
+  Stack unit
+  (requires fun h -> live_multi h result /\ live h hbuf /\
+    internally_disjoint result  /\ disjoint_multi result hbuf)
+  (ensures  fun h0 _ h1 -> modifies_multi result h0 h1 /\
+    as_seq_multi h1 result == SpecVec.emit #a #m (as_seq h0 hbuf))
+
 #push-options "--z3rlimit 700"
 let emit8 #a #m hbuf result =
   let h0 = ST.get() in
   let (b0,(b1,(b2,(b3,(b4,(b5,(b6,b7))))))) = NTup.tup8 result in
   assert (internally_disjoint8 b0 b1 b2 b3 b4 b5 b6 b7);
   copy b0 (sub hbuf 0ul (hash_len a));
-  copy b1 (sub hbuf (8ul *. word_len a) (hash_len a));
-  copy b2 (sub hbuf (16ul *. word_len a) (hash_len a));
-  copy b3 (sub hbuf (24ul *. word_len a) (hash_len a));
+  copy b1 (sub hbuf (8ul *! word_len a) (hash_len a));
+  copy b2 (sub hbuf (16ul *! word_len a) (hash_len a));
+  copy b3 (sub hbuf (24ul *! word_len a) (hash_len a));
   let h1 = ST.get() in
   assert (modifies (loc b0 |+| loc b1 |+| loc b2 |+| loc b3) h0 h1);
-  copy b4 (sub hbuf (32ul *. word_len a) (hash_len a));
-  copy b5 (sub hbuf (40ul *. word_len a) (hash_len a));
-  copy b6 (sub hbuf (48ul *. word_len a) (hash_len a));
-  copy b7 (sub hbuf (56ul *. word_len a) (hash_len a));
+  copy b4 (sub hbuf (32ul *! word_len a) (hash_len a));
+  copy b5 (sub hbuf (40ul *! word_len a) (hash_len a));
+  copy b6 (sub hbuf (48ul *! word_len a) (hash_len a));
+  copy b7 (sub hbuf (56ul *! word_len a) (hash_len a));
   let h1 = ST.get() in
   assert (as_seq h1 b0 == LSeq.sub (as_seq h0 hbuf) 0 (hash_length a));
   assert (as_seq h1 b1 == LSeq.sub (as_seq h0 hbuf) (8 * word_length a) (hash_length a));
@@ -1051,16 +758,16 @@ let emit8 #a #m hbuf result =
 #pop-options
 
 
-inline_for_extraction
-val emit: #a:sha2_alg -> #m:m_spec ->
-          hbuf: lbuffer uint8 (size (lanes a m) *. 8ul *. word_len a) ->
-          result:multibuf (lanes a m) (hash_len a) ->
-    Stack unit
-    (requires (fun h -> live_multi h result /\ live h hbuf /\
-                      internally_disjoint result /\ disjoint_multi result hbuf))
-    (ensures (fun h0 _ h1 -> modifies_multi result h0 h1 /\
-                           as_seq_multi h1 result ==
-                           SpecVec.emit #a #m (as_seq h0 hbuf)))
+inline_for_extraction noextract
+val emit: #a:sha2_alg -> #m:m_spec
+  -> hbuf: lbuffer uint8 (size (lanes a m) *! 8ul *! word_len a)
+  -> result:multibuf (lanes a m) (hash_len a) ->
+  Stack unit
+  (requires fun h -> live_multi h result /\ live h hbuf /\
+    internally_disjoint result /\ disjoint_multi result hbuf)
+  (ensures  fun h0 _ h1 -> modifies_multi result h0 h1 /\
+    as_seq_multi h1 result == SpecVec.emit #a #m (as_seq h0 hbuf))
+
 let emit #a #m hbuf result =
   match lanes a m with
   | 1 -> emit1 #a #m hbuf result
@@ -1069,157 +776,108 @@ let emit #a #m hbuf result =
   | _ -> admit()
 
 
+noextract
+let preserves_disjoint_multi #lanes #len #len' (b:multibuf lanes len) (r:multibuf lanes len') =
+    (forall a l (x:lbuffer a l). disjoint_multi b x ==> disjoint_multi r x)
+
+
+inline_for_extraction noextract
+let get_multiblock_t (a:sha2_alg) (m:m_spec) =
+    len:size_t
+  -> b:multibuf (lanes a m) len
+  -> i:size_t{v i < v len / block_length a} ->
+  Stack (multibuf (lanes a m) (block_len a))
+  (requires fun h -> live_multi h b)
+  (ensures  fun h0 r h1 -> h0 == h1 /\ live_multi h1 r /\ preserves_disjoint_multi b r /\
+    as_seq_multi h1 r == SpecVec.get_multiblock_spec (v len) (as_seq_multi h0 b) (v i))
+
+
+inline_for_extraction noextract
+val get_multiblock: #a:sha2_alg -> #m:m_spec -> get_multiblock_t a m
 let get_multiblock #a #m len b i =
   let h0 = ST.get() in
   match lanes a m with
-  | 1 -> let b0 = NTup.tup1 b in
-         let b' = sub b0 (i *. block_len a) (block_len a) in
-         let mb' = NTup.ntup1 b' in
-         let h1 = ST.get() in
-         NTup.eq_intro (as_seq_multi h1 mb')
-                       (SpecVec.get_multiblock_spec #a #m (v len) (as_seq_multi h0 b) (v i));
-         mb'
-  | 4 -> let (b0,(b1,(b2,b3))) = NTup.tup4 b in
-         let bl0 = sub b0 (i *. block_len a) (block_len a) in
-         let bl1 = sub b1 (i *. block_len a) (block_len a) in
-         let bl2 = sub b2 (i *. block_len a) (block_len a) in
-         let bl3 = sub b3 (i *. block_len a) (block_len a) in
-         let mb = NTup.ntup4 (bl0, (bl1, (bl2, bl3))) in
-         let h1 = ST.get() in
-         NTup.eq_intro (as_seq_multi h1 mb)
-                       (SpecVec.get_multiblock_spec #a #m (v len) (as_seq_multi h0 b) (v i));
-         mb
-  | 8 -> let (b0,(b1,(b2,(b3,(b4,(b5,(b6,b7))))))) = NTup.tup8 b in
-         let bl0 = sub b0 (i *. block_len a) (block_len a) in
-         let bl1 = sub b1 (i *. block_len a) (block_len a) in
-         let bl2 = sub b2 (i *. block_len a) (block_len a) in
-         let bl3 = sub b3 (i *. block_len a) (block_len a) in
-         let bl4 = sub b4 (i *. block_len a) (block_len a) in
-         let bl5 = sub b5 (i *. block_len a) (block_len a) in
-         let bl6 = sub b6 (i *. block_len a) (block_len a) in
-         let bl7 = sub b7 (i *. block_len a) (block_len a) in
-         let mb = NTup.ntup8 (bl0, (bl1, (bl2, (bl3, (bl4, (bl5, (bl6, bl7))))))) in
-         let h1 = ST.get() in
-         NTup.eq_intro (as_seq_multi h1 mb)
-                       (SpecVec.get_multiblock_spec #a #m (v len) (as_seq_multi h0 b) (v i));
-         mb
+  | 1 ->
+    let b0 = NTup.tup1 b in
+    let b' = sub b0 (i *! block_len a) (block_len a) in
+    let mb' = NTup.ntup1 b' in
+    let h1 = ST.get() in
+    NTup.eq_intro (as_seq_multi h1 mb') (SpecVec.get_multiblock_spec #a #m (v len) (as_seq_multi h0 b) (v i));
+    mb'
+  | 4 ->
+    let (b0,(b1,(b2,b3))) = NTup.tup4 b in
+    let bl0 = sub b0 (i *! block_len a) (block_len a) in
+    let bl1 = sub b1 (i *! block_len a) (block_len a) in
+    let bl2 = sub b2 (i *! block_len a) (block_len a) in
+    let bl3 = sub b3 (i *! block_len a) (block_len a) in
+    let mb = NTup.ntup4 (bl0, (bl1, (bl2, bl3))) in
+    let h1 = ST.get() in
+    NTup.eq_intro (as_seq_multi h1 mb) (SpecVec.get_multiblock_spec #a #m (v len) (as_seq_multi h0 b) (v i));
+    mb
+  | 8 ->
+    let (b0,(b1,(b2,(b3,(b4,(b5,(b6,b7))))))) = NTup.tup8 b in
+    let bl0 = sub b0 (i *! block_len a) (block_len a) in
+    let bl1 = sub b1 (i *! block_len a) (block_len a) in
+    let bl2 = sub b2 (i *! block_len a) (block_len a) in
+    let bl3 = sub b3 (i *! block_len a) (block_len a) in
+    let bl4 = sub b4 (i *! block_len a) (block_len a) in
+    let bl5 = sub b5 (i *! block_len a) (block_len a) in
+    let bl6 = sub b6 (i *! block_len a) (block_len a) in
+    let bl7 = sub b7 (i *! block_len a) (block_len a) in
+    let mb = NTup.ntup8 (bl0, (bl1, (bl2, (bl3, (bl4, (bl5, (bl6, bl7))))))) in
+    let h1 = ST.get() in
+    NTup.eq_intro (as_seq_multi h1 mb) (SpecVec.get_multiblock_spec #a #m (v len) (as_seq_multi h0 b) (v i));
+    mb
   | _ -> admit()
 
 
+inline_for_extraction noextract
+let get_multilast_t (a:sha2_alg) (m:m_spec) =
+    len:size_t
+  -> b:multibuf (lanes a m) len ->
+  Stack (multibuf (lanes a m) (len %. block_len a))
+  (requires fun h -> live_multi h b)
+  (ensures  fun h0 r h1 -> h0 == h1 /\ live_multi h1 r /\ preserves_disjoint_multi b r /\
+    as_seq_multi h1 r == SpecVec.get_multilast_spec #a #m (v len) (as_seq_multi h0 b))
 
+inline_for_extraction noextract
+val get_multilast: #a:sha2_alg -> #m:m_spec -> get_multilast_t a m
 #push-options "--z3rlimit 300"
 let get_multilast #a #m len b =
   let h0 = ST.get() in
   let rem = len %. block_len a in
   assert (v (len -! rem) == v len - v rem);
   match lanes a m with
-  | 1 -> let b0 = NTup.tup1 b in
-         let b' = sub b0 (len -! rem) rem in
-         let mb' = NTup.ntup1 b' in
-         let h1 = ST.get() in
-         NTup.eq_intro (as_seq_multi h1 mb')
-                       (SpecVec.get_multilast_spec #a #m (v len) (as_seq_multi h0 b));
-         mb'
-  | 4 -> let (b0,(b1,(b2,b3))) = NTup.tup4 b in
-         let bl0 = sub b0 (len -! rem) rem in
-         let bl1 = sub b1 (len -! rem) rem in
-         let bl2 = sub b2 (len -! rem) rem in
-         let bl3 = sub b3 (len -! rem) rem in
-         let mb = NTup.ntup4 (bl0, (bl1, (bl2, bl3))) in
-         let h1 = ST.get() in
-         NTup.eq_intro (as_seq_multi h1 mb)
-                       (SpecVec.get_multilast_spec #a #m (v len) (as_seq_multi h0 b));
-         mb
-  | 8 -> let (b0,(b1,(b2,(b3,(b4,(b5,(b6,b7))))))) = NTup.tup8 b in
-         let bl0 = sub b0 (len -! rem) (rem) in
-         let bl1 = sub b1 (len -! rem) (rem) in
-         let bl2 = sub b2 (len -! rem) (rem) in
-         let bl3 = sub b3 (len -! rem) (rem) in
-         let bl4 = sub b4 (len -! rem) (rem) in
-         let bl5 = sub b5 (len -! rem) (rem) in
-         let bl6 = sub b6 (len -! rem) (rem) in
-         let bl7 = sub b7 (len -! rem) (rem) in
-         let mb = NTup.ntup8 (bl0, (bl1, (bl2, (bl3, (bl4, (bl5, (bl6, bl7))))))) in
-         let h1 = ST.get() in
-         NTup.eq_intro (as_seq_multi h1 mb)
-                       (SpecVec.get_multilast_spec #a #m (v len) (as_seq_multi h0 b));
-         mb
-  | _ -> admit()
-#pop-options
-
-#push-options "--z3rlimit 200"
-let update_nblocks #a #m upd len b st =
-    let blocks = len /. block_len a in
-    let h0 = ST.get() in
-    loop1 h0 blocks st
-      (fun h -> SpecVec.update_block #a #m (v len) (as_seq_multi h0 b))
-      (fun i ->
-        Lib.LoopCombinators.unfold_repeati (v blocks) (SpecVec.update_block #a #m (v len) (as_seq_multi h0 b)) (as_seq h0 st) (v i);
-        let h0' = ST.get() in
-        let mb = get_multiblock len b i in
-        upd mb st;
-        let h1 = ST.get() in
-        assert (modifies (loc st) h0 h1);
-        NTup.eq_intro (as_seq_multi h0' b) (as_seq_multi h0 b);
-        assert (as_seq h1 st == SpecVec.update_block #a #m (v len) (as_seq_multi h0 b) (v i) (as_seq h0' st)))
-#pop-options
-
-
-#push-options "--z3rlimit 100"
-let finish #a #m st h =
-  let h0 = ST.get() in
-  push_frame();
-  let hbuf = create (size (lanes a m) *. 8ul *. word_len a) (u8 0) in
-  let h1 = ST.get() in
-  store_state st hbuf;
-  emit hbuf h;
-  let h2 = ST.get() in
-  assert (modifies (loc_multi h |+| loc st |+| loc hbuf) h1 h2);
-  assert (as_seq_multi h2 h == SpecVec.finish #a #m (as_seq h0 st));
-  pop_frame();
-  let h3 = ST.get() in
-  assert (modifies (loc_multi h |+| loc st) h0 h3);
-  NTup.eq_intro (as_seq_multi h2 h) (as_seq_multi h3 h);
-  assert (as_seq_multi h2 h == as_seq_multi h3 h);
-  assert (as_seq_multi h3 h == SpecVec.finish #a #m (as_seq h0 st))
-#pop-options
-
-
-#push-options "--z3rlimit 500"
-let hash #a #m upd h len b =
-    let init_h0 = ST.get() in
-    push_frame();
-    let h0 = ST.get() in
-    NTup.eq_intro (as_seq_multi h0 b) (as_seq_multi init_h0 b);
-    let st = alloc a m in
-    init #a #m st;
+  | 1 ->
+    let b0 = NTup.tup1 b in
+    let b' = sub b0 (len -! rem) rem in
+    let mb' = NTup.ntup1 b' in
     let h1 = ST.get() in
-    assert (modifies (loc st) h0 h1);
-    assert (as_seq h1 st == SpecVec.init a m);
-    NTup.eq_intro (as_seq_multi h1 b) (as_seq_multi h0 b);
-    let rem = len %. block_len a in
-    let len' : len_t a = Lib.IntTypes.cast #U32 #PUB (len_int_type a) PUB len in
-    update_nblocks #a #m upd len b st;
-    let h2 = ST.get() in
-    assert (modifies (loc st) h0 h2);
-    assert (as_seq h2 st == SpecVec.update_nblocks (v len) (as_seq_multi h0 b) (as_seq h1 st));
-    NTup.eq_intro (as_seq_multi h2 b) (as_seq_multi h0 b);
-    let lb: multibuf (lanes a m) rem = get_multilast len b in
-    let h3 = ST.get() in
-    assert (h2 == h3);
-    assert (as_seq_multi h3 lb == SpecVec.get_multilast_spec #a #m (v len) (as_seq_multi h2 b));
-    assert (preserves_disjoint_multi b lb);
-    assert (disjoint_multi lb st);
-    update_last #a #m upd len' rem lb st;
-    let h4 = ST.get() in
-    assert (modifies (loc st) h0 h4);
-    assert (as_seq h4 st == SpecVec.update_last len' (v rem) (as_seq_multi h3 lb) (as_seq h3 st));
-    finish #a #m st h;
-    let h5 = ST.get() in
-    assert (modifies (loc_multi h |+| loc st) h0 h5);
-    assert (as_seq_multi h5 h == SpecVec.finish #a #m (as_seq h4 st));
-    assert (as_seq_multi h5 h == SpecVec.hash #a #m (v len) (as_seq_multi h0 b));
-    pop_frame();
-    let h6 = ST.get() in
-    NTup.eq_intro (as_seq_multi h6 h) (as_seq_multi h5 h)
+    NTup.eq_intro (as_seq_multi h1 mb') (SpecVec.get_multilast_spec #a #m (v len) (as_seq_multi h0 b));
+    mb'
+  | 4 ->
+    let (b0,(b1,(b2,b3))) = NTup.tup4 b in
+    let bl0 = sub b0 (len -! rem) rem in
+    let bl1 = sub b1 (len -! rem) rem in
+    let bl2 = sub b2 (len -! rem) rem in
+    let bl3 = sub b3 (len -! rem) rem in
+    let mb = NTup.ntup4 (bl0, (bl1, (bl2, bl3))) in
+    let h1 = ST.get() in
+    NTup.eq_intro (as_seq_multi h1 mb) (SpecVec.get_multilast_spec #a #m (v len) (as_seq_multi h0 b));
+    mb
+  | 8 ->
+    let (b0,(b1,(b2,(b3,(b4,(b5,(b6,b7))))))) = NTup.tup8 b in
+    let bl0 = sub b0 (len -! rem) (rem) in
+    let bl1 = sub b1 (len -! rem) (rem) in
+    let bl2 = sub b2 (len -! rem) (rem) in
+    let bl3 = sub b3 (len -! rem) (rem) in
+    let bl4 = sub b4 (len -! rem) (rem) in
+    let bl5 = sub b5 (len -! rem) (rem) in
+    let bl6 = sub b6 (len -! rem) (rem) in
+    let bl7 = sub b7 (len -! rem) (rem) in
+    let mb = NTup.ntup8 (bl0, (bl1, (bl2, (bl3, (bl4, (bl5, (bl6, bl7))))))) in
+    let h1 = ST.get() in
+    NTup.eq_intro (as_seq_multi h1 mb) (SpecVec.get_multilast_spec #a #m (v len) (as_seq_multi h0 b));
+    mb
+  | _ -> admit()
 #pop-options
